Make notational guarini work

src/chess/algebraic.lean
@@ -1,7 +1,11 @@
 import chess.piece
 import chess.algebraic.utils
+import chess.move.description
 
 open chess
+
+def parse_to_some {α : Type} (p : parser α) : string → option α :=
+sum.elim (λ _, none) some ∘ parser.run_string p
 
 namespace chess
 
@@ -25,93 +29,133 @@ def char_symbol : piece → char
 | ♘ := 'N'
 | ♙ := 'P'
 
-def piece_repr : piece → string
-| ♔ := "♔"
-| ♕ := "♕"
-| ♖ := "♖"
-| ♗ := "♗"
-| ♘ := "♘"
-| ♙ := "♙"
-
-abbreviation promotions : Type := {p : piece // p = ♕ ∨ p = ♖ ∨ p = ♗ ∨ p = ♘}
-
-instance : has_repr piece := ⟨piece_repr⟩
-
-def parser' (x : piece) : parser piece :=
-(ch x.char_symbol <|> ch x.unicode_symbol) $> x
+def parser' : piece → parser piece :=
+λ (x : piece), (ch x.char_symbol <|> ch x.unicode_symbol) $> x
 
 def promotions.parser' : parser piece :=
 decorate_error "<promotions>" $ mfirst parser' [queen, rook, bishop, knight]
 
--- lemma promotions.parser'_not_king (cb n) (h : promtions.parser' cb n ≠ parse_result.fail): promotions.parser' cb n
+lemma mem_of_mfirst_map_const_eq_done {α β} {f : α → parser β} {l : list α} {a}
+  (h : a ∈ mfirst (λ x, f x $> x) l) : a ∈ l :=
+begin
+  obtain ⟨p, hp, hp'⟩ := mem_of_mfirst h,
+  simp only [list.mem_map, list.map_eq_map] at hp,
+  obtain ⟨x, hx, rfl⟩ := hp,
+  simp only [mem_map_const_iff] at hp',
+  exact hp'.left ▸ hx
+end
+
+lemma promotions.parser'_mem' {p : piece} (h : p ∈ promotions.parser') :
+  p ∈ [queen, rook, bishop, knight] :=
+begin
+  simp only [promotions.parser', parser', mem_decorate_error_iff] at h,
+  exact mem_of_mfirst_map_const_eq_done h
+end
+
+def promotions.parser : parser promotions :=
+parser.attach promotions.parser' (λ p h, by {
+  have H := promotions.parser'_mem' h,
+  simp only [list.mem_cons_iff, list.mem_singleton] at H,
+  exact H
+})
 
 def parser : parser piece :=
 decorate_error "<piece>" $ mfirst parser' [king, queen, rook, bishop, knight, pawn]
 
 end piece
 
-@[derive [decidable_eq, fintype]]
-inductive capture
-| capture
-| noncapture
+instance castle_has_repr : has_repr castle := ⟨castle.repr⟩
 
-def capture.repr : capture → string
-| capture.capture := "capture"
-| capture.noncapture := "noncapture"
+variables {m n : Type}
+variables [has_zero m] [has_one m] [has_add m]
+variables [has_zero n] [has_one n] [has_add n]
 
-instance capture_has_repr : has_repr capture := ⟨capture.repr⟩
-
-variables {α β : Type} [has_zero α] [has_one α] [has_add α] [has_zero β] [has_one β] [has_add β]
-
-def file.parser' : parser α := numeral.char _ 'a' 'z'
-def file.parser [fintype α] : parser α := numeral.char.of_fintype _ 'a'
-def rank.parser' : parser α := numeral.from_one α
-def rank.parser [fintype α] : parser α := numeral.from_one.of_fintype α
-def square.parser' : parser (α × β) :=
+def file.parser' : parser m := numeral.char _ 'a' 'z'
+def file.parser [fintype m] : parser m := numeral.char.of_fintype _ 'a'
+def rank.parser' : parser m := numeral.from_one m
+def rank.parser [fintype m] : parser m := numeral.from_one.of_fintype m
+def square.parser' : parser (m × n) :=
 (λ x y, ⟨y, x⟩) <$> file.parser' <*> rank.parser'
-def square.parser [fintype α] [fintype β] : parser (α × β) :=
+def square.parser [fintype m] [fintype n] : parser (m × n) :=
 (λ x y, ⟨y, x⟩) <$> file.parser <*> rank.parser
-def square.parser.optional [fintype α] [fintype β] : parser (option α × option β) :=
-(λ x y, ⟨y, x⟩) <$> (some <$> file.parser <|> pure none) <*> (some <$> rank.parser <|> pure none)
+def square.parser.optional [fintype m] [fintype n] : parser (option m × option n) :=
+(λ x y, ⟨y, x⟩) <$> (file.parser.option) <*> (rank.parser.option)
 def capture.parser : parser capture :=
-ch 'x' $> capture.capture <|> pure capture.noncapture
+ch 'x' $> capture.capture
+def castle.parser : parser castle :=
+(str "O-O-O" $> castle.queens) <|> (str "O-O" $> castle.kings)
 
-variables (α β)
+variables [fintype m] [fintype n] [decidable_eq m] [decidable_eq n] [linear_order m] [linear_order n]
 
-structure move.description :=
-(figure : piece)
-(from_sq : (option α × option β))
-(to_sq : (α × β))
-(capture : capture)
+-- in this order because absence of the from-square and capture will parse the to-square as
+-- from-square, and fail the parser
+def move.not_pawn.parser : parser (move.description.chess m n) :=
+try ((λ fig fsq cap tsq, ⟨⟨fig, fsq, tsq⟩, cap, none⟩) <$>
+  piece.parser <*> square.parser.optional <*> capture.parser.option <*> square.parser) <|>
+  (λ fig cap tsq, ⟨⟨fig, (none, none), tsq⟩, cap, none⟩) <$>
+    piece.parser <*> capture.parser.option <*> square.parser
 
-instance move.description.has_repr [has_repr α] [has_repr β] : has_repr (move.description α β) :=
-⟨λ ⟨p, fsq, tsq, c⟩, string.intercalate " " [repr p, repr fsq, repr tsq, repr c]⟩
+def move.pawn.push.parser : parser (move.description.chess m n) :=
+(λ tsq prom, ⟨⟨pawn, (none, none), tsq⟩, none, prom⟩) <$>
+  square.parser <*> piece.promotions.parser.option
 
-structure pawn.capture.description extends move.description α β :=
-(promoted : {p : piece // p ≠ pawn ∧ p ≠ king})
+def move.pawn.capture.parser : parser (move.description.chess m n) :=
+(λ f r cap tsq prom, ⟨⟨pawn, (r, f), tsq⟩, cap, prom⟩) <$>
+  (some <$> file.parser) <*> rank.parser.option <*> (some <$> capture.parser) <*> square.parser <*>
+  piece.promotions.parser.option
 
-variables {α β}
+-- in this order because the push parser is strictly a prefix of the capture parser
+def move.pawn.parser : parser (move.description.chess m n) :=
+mfirst try [move.pawn.push.parser, move.pawn.capture.parser]
 
-def move.parser [fintype α] [fintype β] : parser (move.description α β) :=
-(λ p fsq c tsq, ⟨p, fsq, tsq, c⟩) <$> piece.parser <*> square.parser.optional <*> capture.parser <*> square.parser
+def move.parser : parser (move.description.chess m n) :=
+mfirst try [move.not_pawn.parser, move.pawn.parser]
 
-#eval run_string (piece.parser) "♗"
-#eval run_string (piece.parser) "K"
-#eval run_string (piece.parser) "N"
-#eval run_string (piece.parser) "x"
-#eval run_string (piece.parser.many) "KQRBNP"
-#eval run_string (piece.parser.many) "KQRBNX"
+def notation.parser : parser unit :=
+one_of ['!', '?', '+', '#'] $> ()
 
-#eval run_string (numeral (fin 300)) "001334"
-#eval run_string (@file.parser' (fin 300) _ _ _) "a"
-#eval run_string (@file.parser (fin 8) _ _ _ _) "a"
-#eval run_string (@file.parser (fin 8) _ _ _ _) "h"
-#eval run_string (@file.parser (fin 8) _ _ _ _) "i"
-#eval run_string (@rank.parser (fin 300) _ _ _ _) "4"
-#eval run_string (@square.parser (fin 300) (fin 300) _ _ _ _ _ _ _ _) "a4"
+instance {α : Type*} [has_repr α] : has_repr (parse_result α) := ⟨
+  λ pr, @parse_result.cases_on _ (λ _, string) pr
+    (λ n a, "done (" ++ repr n ++ "): " ++ repr a)
+    (λ n a, "fail (" ++ repr n ++ "): " ++ repr a.to_list)
+⟩
 
-#eval run_string capture.parser ""
+def general.parser : parser (castle ⊕ move.description.chess (fin 8) (fin 8)) :=
+(sum.inl <$> castle.parser) <|> (sum.inr <$> (move.parser <* notation.parser.option))
 
-#eval run_string (@move.parser (fin 8) (fin 8) _ _ _ _ _ _ _ _) "Qd5xc8"
+#eval
+(parse_to_some
+  ((parser.nat *> (ch '.') *> (ch ' ')) *> (
+    (sep_by1
+      (parser.nat *> (ch '.') *> (ch ' ').option $> ())
+      (prod.mk <$>
+        (general.parser <* (ch ' ').option) <*>
+        ((general.parser <* (ch ' ').option).try <|>
+          ((parser.nat *> ch '-' <* parser.nat) $> sum.inl castle.kings))))
+        -- quick way to parse "1-0" scores
+  ))
+(
+  "1. e4 c6 2. d4 d5 3. Nc3 dxe4 4. Nxe4 Nf6 5. Qd3 e5 6. dxe5
+Qa5+ 7. Bd2 Qxe5 8. O-O-O Nxe4 9. Qd8+ Kxd8 10. Bg5+ Kc7
+11. Bd8# 1-0".to_list.map (λ c, if c = '\n' then ' ' else c)
+).as_string)
+
+#eval
+(parse_to_some
+  ((parser.nat *> (ch '.') *> (ch ' ')) *> (
+    (sep_by1
+      (parser.nat *> (ch '.') *> (ch ' ').option $> ())
+      (prod.mk <$>
+        (general.parser <* (ch ' ').option) <*>
+        ((general.parser <* (ch ' ').option).try <|>
+          ((parser.nat *> ch '-' <* parser.nat) $> sum.inl castle.kings))))
+        -- quick way to parse "1-0" scores
+  ))
+(
+  "1. e4 e5 2. Nf3 Nc6 3. Bb5 Nf6 4. O-O d6 5. d4 Nxe4 6. d5 a6
+7. Bd3 Nf6 8. dxc6 e4 9. Re1 d5 10. Be2 exf3 11. cxb7 Bxb7
+12. Bb5# 1-0"
+  .to_list.map (λ c, if c = '\n' then ' ' else c)
+).as_string)
 
 end chess
