src/guarini.lean
@@ -1,5 +1,5 @@
-import chess.move.legal
 import chess.notation
+import chess.algebraic.move
 
 /-!
 
@@ -75,6 +75,46 @@ def guarini_seq : chess.move.sequence.legal :=
   ((2, 1), (0, 0)),
   ((1, 2), (2, 0))] }
 
+
+def guarini_algebraic : list string :=
+  [
+    "Nab1",
+    "N3a2",
+    "Nbc3",
+    "Ncb3",
+    "Nac2",
+    "Nca3",
+    "Nab1",
+    "Nba1",
+    "Nac2",
+    "Nac1",
+    "Ncb3",
+    "Nca2",
+    "Nac1",
+    "Nbc3",
+    "Nba1",
+    "Nca3"
+  ]
+
+#eval starting_position.run_move_sequence_no_capture guarini_algebraic
+/-
+(some ♞, ♞, ♘, ♘;
+
+♘, ＿, ♘;
+＿, ＿, ＿;
+♞, ＿, ♞)
+-/
+
+#eval some ending_position
+/-
+(some ♘, ♘, ♞, ♞;
+
+♘, ＿, ♘;
+＿, ＿, ＿;
+♞, ＿, ♞)
+-/
+
+
 def first_move : chess.move starting_position :=
 let pair := guarini_seq.elements.nth_le 0 dec_trivial in ⟨pair.fst, pair.snd, dec_trivial, dec_trivial⟩
 
@@ -87,5 +127,12 @@ example : ∀ ix (hix : ix < guarini_seq.elements.length),
 
 lemma guarini : starting_position.has_sequence_to ending_position :=
 ⟨guarini_seq.elements.length, guarini_seq.to_sequence, dec_trivial⟩
+
+lemma guarini_SAN :
+  ((starting_position.run_move_sequence_no_capture guarini_algebraic).map chess.board.reduce) =
+  some ending_position.reduce := dec_trivial
+  /-
+deep recursion was detected at 'replace' (potential solution: increase stack space in your system)
+-/
 
 -- Graph-equivalence
