src/chess/algebraic/move.lean
@@ -1,0 +1,32 @@
+import chess.move.description
+import chess.algebraic
+
+open chess
+
+namespace chess
+
+namespace board
+
+variables {m n : Type} {i : ℕ}
+
+variables [has_zero m] [has_one m] [has_add m]
+variables [has_zero n] [has_one n] [has_add n]
+variables [fintype m] [decidable_eq m] [linear_order m]
+variables [fintype n] [decidable_eq n] [linear_order n]
+
+def run_move_sequence_no_capture (b : board m n (fin i) colored_piece) (l : list string) :
+  option (board m n (fin i) colored_piece) :=
+mfoldl
+  (λ B str, parse_to_some move.parser str >>= λ desc, (B.run_move desc).pbind
+    (λ pair hp, desc.capture.pbind_with
+      (λ h, chess.move.perform_move (
+        ⟨pair.fst, pair.snd, desc.occupied_start B hp, desc.unoccupied_end_of_no_capture B hp h⟩
+        : chess.move B))
+      (λ _ _, none)
+    )
+  )
+b l
+
+end board
+
+end chess
