src/chess/move/description.lean
@@ -1,0 +1,110 @@
+import chess.move.legal
+
+open chess
+
+namespace chess
+
+variables (m n : Type)
+
+variables [fintype m] [decidable_eq m] [linear_order m]
+variables [fintype n] [decidable_eq n] [linear_order n]
+
+structure move.description (K : Type*) :=
+(figure : K)
+(from_sq : (option m × option n))
+(to_sq : (m × n))
+
+structure move.description.chess extends move.description m n piece :=
+(capture : option capture)
+(promoted : option promotions)
+
+instance move.description.has_repr [has_repr m] [has_repr n] :
+  has_repr (move.description.chess m n) :=
+⟨λ ⟨⟨p, fsq, tsq⟩, cap, prom⟩, string.intercalate " "
+  [repr p, repr fsq, repr tsq, repr cap, repr prom]⟩
+
+section run_move
+
+variables {m n}
+
+variables {i : ℕ} (b : board m n (fin i) chess.colored_piece)
+  (d : move.description m n chess.piece)
+  (d' : move.description.chess m n)
+
+namespace board
+
+def run_move' : option ((m × n) × (m × n)) :=
+option.map (λ ix, (b.pos_from ix, d.to_sq))
+  (list.exactly_one (list.filter (λ ix,
+    ((chess.colored_piece.piece ∘ b.pieces) ix) = d.figure ∧
+    (d.from_sq.fst = none ∨ some (b.pos_from ix).fst = d.from_sq.fst) ∧
+    (d.from_sq.snd = none ∨ some (b.pos_from ix).snd = d.from_sq.snd) ∧
+    (chess.piece.move_rule ((chess.colored_piece.piece ∘ b.pieces) ix)
+    (b.pos_from ix) d.to_sq)
+  ) (list.fin_range i)))
+
+def run_move : option ((m × n) × (m × n)) :=
+if d'.capture = none
+  then if b.contents d'.to_description.to_sq = none
+    then b.run_move' d'.to_description
+    else none
+  else if b.contents d'.to_description.to_sq = none
+    then none
+    else b.run_move' d'.to_description
+
+end board
+
+open board
+
+lemma move.description.occupied_start {pair : ((m × n) × (m × n))} (h : pair ∈ b.run_move' d) :
+  b.contents.occupied_at pair.fst :=
+begin
+  obtain ⟨x, y⟩ := pair,
+  simp only [run_move', option.mem_def, prod.mk.inj_iff, function.comp_app, option.map_eq_some',
+             list.exactly_one_some] at h,
+  obtain ⟨ix, h, rfl, rfl⟩ := h,
+  exact playfield.pos_from_occupied ix _ _
+end
+
+lemma move.description.chess.occupied_start {pair : ((m × n) × (m × n))} (h : pair ∈ b.run_move d') :
+  b.contents.occupied_at pair.fst :=
+begin
+  simp only [run_move, option.mem_def] at h,
+  split_ifs at h,
+  { exact d'.to_description.occupied_start b h },
+  { exact false.elim h },
+  { exact false.elim h },
+  { exact d'.to_description.occupied_start b h }
+end
+
+lemma move.description.chess.unoccupied_end_of_no_capture {pair : ((m × n) × (m × n))}
+  (h : pair ∈ b.run_move d') (h' : d'.capture = none) :
+  ¬ b.contents.occupied_at pair.snd :=
+begin
+  obtain ⟨x, y⟩ := pair,
+  simp only [run_move, run_move', option.mem_def, function.comp_app, h', if_true,
+              eq_self_iff_true] at h,
+  split_ifs at h with H H,
+  { simp only [prod.mk.inj_iff, option.map_eq_some', list.head'_cons, list.exactly_one_some] at h,
+    obtain ⟨ix, h, rfl, rfl⟩ := h,
+    rintro ⟨p, hp⟩,
+    simpa only [H] using hp },
+  { exact false.elim h }
+end
+
+lemma move.description.chess.occupied_end_of_capture {pair : ((m × n) × (m × n))}
+  (h : pair ∈ b.run_move d') (h' : d'.capture = some capture.capture) :
+  b.contents.occupied_at pair.snd :=
+begin
+  obtain ⟨x, y⟩ := pair,
+  simp only [run_move, run_move', option.mem_def, function.comp_app, h', if_false] at h,
+  split_ifs at h with H H,
+  { exact false.elim h },
+  { simp only [prod.mk.inj_iff, option.map_eq_some', list.head'_cons, list.exactly_one_some] at h,
+    obtain ⟨ix, h, rfl, rfl⟩ := h,
+    exact playfield.occupied_at_of_ne H }
+end
+
+end run_move
+
+end chess
